Adapt erasure plugin

erasure/theories/EWtAst.v
@@ -1,9 +1,11 @@
 (* Distributed under the terms of the MIT license. *)
-From Coq Require Import ssreflect.
+From Coq Require Import ssreflect ssrbool.
 From MetaCoq.Template Require Import utils BasicAst Universes.
 From MetaCoq.PCUIC Require Import PCUICPrimitive.
-From MetaCoq.Erasure Require Import EAst ECSubst ELiftSubst ETyping EEtaExpanded.
+From MetaCoq.Erasure Require Import EAst EAstUtils ECSubst ELiftSubst ETyping.
+(* EEtaExpanded.*)
 From Equations Require Import Equations.
+Set Equations Transparent.
 
 Import MCMonadNotation.
 
@@ -102,31 +104,265 @@ Section WellScoped.
     all:rtoProp; intuition eauto.
   Qed.
 
-  Definition eterm n := { t : EAst.term | well_scoped n t && isEtaExp Σ t }.
-
-  
+  Definition eterm n := { t : EAst.term | well_scoped n t }.
+  Definition eterm_term {n} (e : eterm n) := proj1_sig e.
+  Definition well_scoped_eterm {n} (e : eterm n) : well_scoped n (eterm_term e) := proj2_sig e.
 End WellScoped.
 
-Module TermSpineView.
+Arguments eterm_term {Σ n}.
 
-  Inductive t (A : Type) : term -> Set :=
-  | tBox       : t EAst.tBox
-  | tRel (n : nat) : t (EAst.tRel n)
-  | tVar (n : ident) : t (EAst.tVar n)
-  | tEvar (n : nat) (e : list A) : t (EAst.tEvar n e)
-  | tLambda n b : t (EAst.tLambda n b)
-  | tLetIn n b b' : t (EAst.tLetIn n b b')
-  | tApp (f : term) (l : list term) (napp : ~~ isApp f) (nnil : l <> nil) : t (mkApps f l)
-  | tConst kn : t (tConst kn)
-  | tConstruct i n : t (tConstruct i n)
-  | tCase ci p brs : t (tCase ci p brs)
-  | tProj p c : t (tProj p c)
-  | tFix mfix idx : t (tFix mfix idx)
-  | tCoFix mfix idx : t (tCoFix mfix idx).
-  Derive Signature for t.
+Coercion eterm_term : eterm >-> term.
+Coercion well_scoped_eterm : eterm >-> is_true.
 
-Definition view : forall x : term, t x :=
-  MkAppsInd.case (P:=fun x => t x)
+Module Constructors.
+  Section Constructors.
+  Context {Σ : global_context} {n : nat}.
+  
+  Program Definition tBox : eterm Σ n := tBox.
+  
+  Program Definition tRel (i : nat) (Hi : i < n) : eterm Σ n := tRel i.
+  Next Obligation. simp well_scoped. eapply Nat.leb_le. lia. Qed.
+  
+  Program Definition tEvar k (l : list (eterm Σ n)) : eterm Σ n := tEvar k (map eterm_term l).
+  Next Obligation. 
+    simp well_scoped. induction l; cbn; simp well_scoped => //.
+    rewrite IHl andb_true_r. exact a. 
+  Qed.
+  
+  Program Definition tLambda na (b : eterm Σ (S n)) : eterm Σ n := tLambda na b.
+  Next Obligation.
+    simp well_scoped. exact b.
+  Qed.
+
+
+  Program Definition tLetIn na (b : eterm Σ n) (b' : eterm Σ (S n)) : eterm Σ n := tLetIn na b b'.
+  Next Obligation.
+    simp well_scoped. apply/andP; split. exact b. exact b'.
+  Qed.
+
+  Program Definition tApp (f : eterm Σ n) (l : list (eterm Σ n)) (napp : ~~ isApp f) (nnil : l <> nil) : eterm Σ n :=
+    mkApps f (map eterm_term l).
+  Next Obligation.
+    induction l using rev_ind => //. 
+    rewrite map_app EAstUtils.mkApps_app /=.
+    simp well_scoped.
+    apply/andP; split.
+    - destruct l; cbn; [exact f|].
+      apply IHl. congruence.
+    - exact x.
+  Qed.
+
+  Program Definition tConst kn (isdecl : declared_constant Σ kn) : eterm Σ n := tConst kn.
+
+  Program Definition tConstruct ind k (isdecl : declared_constructor Σ ind k) : eterm Σ n := tConstruct ind k.
+  
+  Program Definition tCase ci (c : eterm Σ n) (brs : list (∑ args : list name, eterm Σ (#|args| + n)))
+    (isdecl : declared_inductive Σ ci.1) : eterm Σ n :=
+    tCase ci c (map (fun br : ∑ args, eterm Σ (#|args| + n) => (br.π1, proj1_sig br.π2)) brs).
+  Next Obligation.
+    simp well_scoped. apply/andP; split.
+    - apply/andP; split => //. exact c.
+    - induction brs; simp well_scoped => //.
+      cbn. rewrite IHbrs andb_true_r. exact a.π2.
+  Qed.
+
+  Program Definition tProj p (c : eterm Σ n) (isdecl : declared_projection Σ p) : eterm Σ n :=
+    tProj p c.
+  Next Obligation.
+    simp well_scoped. rewrite isdecl; exact c.
+  Qed.
+  Definition edefs := ∑ mfix : mfixpoint term, well_scoped_mfix Σ (#|mfix| + n) mfix.
+
+  Program Definition tFix (mfix : edefs) idx : eterm Σ n := (tFix mfix.π1 idx).
+  Next Obligation.
+    simp well_scoped. exact mfix.π2.
+  Qed.
+  
+  Program Definition tCoFix (mfix : edefs) idx : eterm Σ n := (tCoFix mfix.π1 idx).
+  Next Obligation.
+    simp well_scoped. exact mfix.π2.
+  Qed.
+  End Constructors.
+End Constructors.
+
+Module View.
+  Section view.
+    Context {Σ : global_context} {n : nat}.
+
+    Inductive t : eterm Σ n -> Set :=
+    | tBox       : t Constructors.tBox
+    | tRel (i : nat) (le : i < n) : t (Constructors.tRel i le)
+    | tEvar (k : nat) l : t (Constructors.tEvar k l)
+    | tLambda na b : t (Constructors.tLambda na b)
+    | tLetIn na b b' : t (Constructors.tLetIn na b b')
+    | tApp (f : eterm Σ n) l (napp : ~~ isApp f) (nnil : l <> nil) : t (Constructors.tApp f l napp nnil)
+    | tConst kn (isdecl : declared_constant Σ kn): t (Constructors.tConst kn isdecl)
+    | tConstruct i k isdecl : t (Constructors.tConstruct i k isdecl)
+    | tCase ci c brs isdecl : t (Constructors.tCase ci c brs isdecl)
+    | tProj p c isdecl : t (Constructors.tProj p c isdecl)
+    | tFix mfix idx : t (Constructors.tFix mfix idx)
+    | tCoFix mfix idx : t (Constructors.tCoFix mfix idx).
+    Derive Signature for t.
+  End view.
+End View.
+    
+
+Lemma well_scoped_irr {Σ n t} (ws ws' : well_scoped Σ n t) : ws = ws'.
+Proof. apply uip. Qed.
+
+Section view.
+  Context {Σ : global_context} {n : nat}.
+
+  Equations? ws_list (l : list term) (ws : well_scoped_terms Σ n l) : list (eterm Σ n) :=
+    | [], _ => []
+    | t :: ts, ws => (exist _ t _) :: ws_list ts _.
+  Proof.
+    all:move/andP: ws => [] //.
+  Qed.
+
+  Lemma ws_list_eq l ws : map eterm_term (ws_list l ws) = l.
+  Proof. funelim (ws_list l ws); cbn; auto. now rewrite H. Qed.
+
+  Equations? ws_brs (l : list (list name × term)) (ws : well_scoped_brs Σ n l) : list (∑ args, eterm Σ (#|args| + n)) :=
+    | [], _ => []
+    | t :: ts, ws => (t.1; exist _ t.2 _) :: ws_brs ts _.
+  Proof.
+    all:move/andP: ws => [] //.
+  Qed.
+
+  Definition ebr_br := (fun br : ∑ args : list name, eterm Σ (#|args| + n) => (br.π1, proj1_sig br.π2)).
+
+  Lemma ws_brs_eq l ws : map ebr_br (ws_brs l ws) = l.
+  Proof. funelim (ws_brs l ws); cbn; auto. rewrite H. destruct t => //. Qed.
+
+  Lemma andb_left {a b} : a && b -> a.
+  Proof.
+    move/andP=>[] //.
+  Qed.
+
+  Lemma andb_right {a b} : a && b -> b.
+  Proof.
+    move/andP=>[] //.
+  Qed.
+
+  Lemma well_scoped_terms_forallb {l} : well_scoped_terms Σ n l = forallb (well_scoped Σ n) l.
+  Proof.
+    induction l; simp well_scoped; auto.
+    now rewrite IHl.
+  Qed.
+
+  Lemma well_scoped_mkApps {f l} : well_scoped Σ n (mkApps f l) -> well_scoped Σ n f && well_scoped_terms Σ n l.
+  Proof.
+    induction l using rev_ind; cbn; auto.
+    - now intros ->.
+    - rewrite mkApps_app /=.
+      move/andP=> [] wfl wx.
+      move/andP: (IHl wfl) => [] => -> wfnl /=.
+      now rewrite well_scoped_terms_forallb forallb_app -well_scoped_terms_forallb /= wfnl wx.
+  Qed.
+
+  Notation " ( x ⧆ y ) " := (exist _ x y).
+
+  Definition view (x : eterm Σ n) : View.t x.
+  Proof.
+    destruct x as [t ws].
+    set (t' := t).
+    destruct t;
+    try solve [evar (ws' : well_scoped Σ n t' = true); rewrite (well_scoped_irr ws ws'); subst ws' t';
+      unshelve econstructor; eauto].
+    - evar (ws' : well_scoped Σ n t' = true); rewrite (well_scoped_irr ws ws'); subst ws' t'.
+      unshelve econstructor. now eapply Nat.leb_le.
+    - cbn in ws; discriminate.
+    - pose proof (ws_list_eq l ws). set(l' := ws_list l ws) in *. clearbody l'.
+      subst t'.
+      revert ws. destruct H.
+      intros ws. set (t' := tEvar _ _).
+      evar (ws' : well_scoped Σ n t' = true); rewrite (well_scoped_irr ws ws'); subst ws' t'.
+      econstructor.
+    - cbn in ws.
+      change t with (eterm_term (exist _ t ws)) in t'.
+      evar (ws' : well_scoped Σ n t' = true); rewrite (well_scoped_irr ws ws'); subst ws' t'.
+      econstructor.
+    - change t2 with (eterm_term (t2 ⧆ andb_right ws)) in t'.
+      change t1 with (eterm_term (t1 ⧆ andb_left ws)) in t'.
+      revert t'.
+      set (prf := andb_left ws).
+      set (prf' := andb_right _). clearbody prf prf'.
+      intros t'.
+      evar (ws' : well_scoped Σ n t' = true).
+      rewrite (well_scoped_irr ws ws'); subst ws' t'.
+      econstructor.
+    - destruct (decompose_app (tApp t1 t2)) eqn:da.
+      move: ws. revert t'.
+      rewrite (decompose_app_inv da).
+      intros t' ws.
+      move: (decompose_app_notApp _ _ _ da).
+      move: (EInduction.decompose_app_app _ _ _ _ da).
+      clear da t1 t2.
+      pose proof (wfa := well_scoped_mkApps ws).
+      pose proof (ws_list_eq l (andb_right wfa)).
+      set(l'' := ws_list l _) in *. clearbody l''.
+      move: ws. revert t'.
+      destruct H.
+      intros t'.
+      change t with (eterm_term (t ⧆ andb_left wfa)) in t'.
+      set (prfa := andb_left wfa) in *. clearbody prfa.
+      intros ws hl ht.
+      evar (ws' : well_scoped Σ n t' = true).
+      rewrite (well_scoped_irr ws ws'); subst ws' t'.
+      unshelve econstructor. exact ht.
+      intros hl'. subst l''. cbn in hl. congruence.
+
+    - destruct p as [ind k].
+      change t with (eterm_term (t ⧆ andb_right (andb_left ws))) in t'.
+      set (prf1 := andb_right _) in t'. clearbody prf1.
+      pose proof (ws_brs_eq _ (andb_right ws)).
+      set (prf2 := andb_right _) in *. clearbody prf2.
+      revert t' ws. destruct H.
+      intros t' ws.
+      evar (ws' : well_scoped Σ n t' = true).
+      rewrite (well_scoped_irr ws ws'); subst ws' t'.
+      unshelve econstructor.
+      cbn. apply (andb_left (andb_left ws)).
+      
+    - change t with (eterm_term (t ⧆ andb_right ws)) in t'.
+      set (prf := andb_right ws) in *. clearbody prf.
+      evar (ws' : well_scoped Σ n t' = true).
+      rewrite (well_scoped_irr ws ws'); subst ws' t'.
+      unshelve econstructor. apply (andb_left ws).
+    - change m with (((m; ws) : Constructors.edefs).π1) in t'.
+      evar (ws' : well_scoped Σ n t' = true).
+      rewrite (well_scoped_irr ws ws'); subst ws' t'.
+      econstructor.
+    - change m with (((m; ws) : Constructors.edefs).π1) in t'.
+      evar (ws' : well_scoped Σ n t' = true).
+      rewrite (well_scoped_irr ws ws'); subst ws' t'.
+      econstructor.
+  Defined.
+
+    -
+    
+    - cbn. eapply View.tBox. econstructor. 
+  | (tRel i; ws) => View.tRel i _
+  | _ => todo "bla".
+    | tVar n => pvar n
+    | tEvar n l => pevar n l
+    | tBox => pbox
+    | tLambda n1 t => plam n1 t
+    | tLetIn n2 t0 t1 => plet n2 t0 t1
+    | tApp t2 t3 with inspect (decompose_app (tApp t2 t3)) := 
+      { | exist _ (t, l) da := 
+        let napp := decompose_app_notApp _ _ _ da in
+        let nonnil := decompose_app_app _ _ _ _ da in
+        rew [P] (eq_sym (decompose_app_inv da)) in papp t l napp nonnil }
+    | tConst k => pconst k
+    | tConstruct i n => pconstruct i n
+    | tCase ina c brs => pcase ina c brs
+    | tProj p c => pproj p c
+    | tFix mfix idx => pfix mfix idx
+    | tCoFix mfix idx => pcofix mfix idx.
+
+  MkAppsInd .case (P:=fun x => t x)
     tBox tRel tVar 
     (fun n l => tEvar n l) 
     (fun n t => tLambda n t)
